theories/Lambda/Polymorphic.v
@@ -1,4 +1,5 @@
 Require Import ExtLib.Data.Vector.
+Require Import ExtLib.Structures.Functor.
 
 Set Implicit Arguments.
 Set Strict Implicit.
@@ -19,5 +20,19 @@ Section poly.
     | S n => fun p a => inst (p (Vector.vector_hd a)) (Vector.vector_tl a)
     end.
 End poly.
+
+Section fmap_polymorphic.
+  Context {Z T U : Type}.
+  Variable f : T -> U.
+  Fixpoint fmap_polymorphic (n : nat)
+  : polymorphic Z n T -> polymorphic Z n U :=
+    match n with
+    | 0 => f
+    | S n => fun x y => fmap_polymorphic n (x y)
+    end.
+End fmap_polymorphic.
+
+Instance Functor_polymorphic Z n : Functor (polymorphic Z n) :=
+{ fmap := fun T U f => @fmap_polymorphic Z T U f n }.
 
 Arguments inst {typ T n} p v : clear implicits, rename.
