theories/Lib/TypeVar.v
@@ -1,0 +1,30 @@
+Require Import ExtLib.Data.Positive.
+Require Import MirrorCore.MTypes.ModularTypes.
+
+Inductive VType : nat -> Type :=
+| tVar : positive -> VType 0.
+
+Definition VType_dec n (a : VType n) : forall b : VType n, {a = b} + {a <> b} :=
+  match a as a in VType n return forall b, {a = b} + {a <> b} with
+  | tVar n => fun b =>
+    match b as b in VType 0 return {tVar n = b} + {tVar n <> b} with
+    | tVar n' => match Pos.eq_dec n n' with
+                 | left pf => left (f_equal _ pf)
+                 | right pf =>
+                   right (fun pf' : tVar n = tVar n' =>
+                            pf match eq_sym pf' in _ = t
+                                     return match t with
+                                            | tVar x => x
+                                            end = n'
+                               with
+                               | eq_refl => eq_refl
+                               end)
+                 end
+    end
+  end.
+
+Instance TSym_VType : TSym VType :=
+{ symbolD n x := match x with
+                 | tVar _ => Empty_set
+                 end
+; symbol_dec := VType_dec }.
